Cm/PiE/SigmaFn.lean
@@ -1,0 +1,93 @@
+/-
+Sigma types feel almost like application.
+
+if you think about it, it feels kinda suboptimal to be doing the order this way.
+
+:: (x : α) (xs : ∀ (x : α), β x)
+
+this is literally reversed application.
+x is the argument, xs is the function.
+
+id : ∀ (α : Type), α → α
+
+:: (α : Type) id
+:: x (:: α id)
+this doesn't really solve the currying issue.
+
+apply : ∀ (α : Type) (β : α → Type) : ∀ (l : ((∀ (x : α), β x) × α)), l.fst l.snd
+
+apply : ∀ (l : ((α : Type) × (β (α : Type) (β : α → Type) (l : ((x : α) × (f : β x))), β l.fst
+
+(:: (x : α) (xs : β x)) : ((x : α) × β x)
+
+what is the purpose of apply?
+apply ((x : α) × β x) into just β x
+
+(:: (x : α) (
+
+observations:
+- we would like to use fully uncurried positional arguments. this makes making the types a BREEZE.
+
+id : ∀ (x : α)
+
+we are being imprecise with how we write ×.
+
+× α β represents the entirety of ((x : α) × β x)
+
+the type of id α x is ::[(Ty m), α, α]
+
+this is
+
+t_id α x = ::[(α : (Ty m)), ::[both, ::[id, Ty m], ::[id, Ty m]]]
+
+so wait what?
+projection gives us the values?
+
+(t_id α x).snd = ::[α, α]
+but then here, α wants to depend on α again, which is fine.
+
+t_id α x = ::[:: id m.succ Ty m, ::[id m.succ, Ty m], ::[id m.succ, Ty m]]
+
+what happens to x?
+
+id.{[m]} : ::[:: id m.succ Ty m, ::[id m.succ, Ty m], ::[id m.succ, Ty m]]
+nil at the end closes the loop?
+
+::[x, α, ::[:: id m.succ Ty m, ::[id m.succ, Ty m], ::[id m.succ, Ty m]]]
+
+there is an extra α here.
+
+- sigma cons seems like absurdly powerful.
+
+but what about checking (α : Ty m)?
+
+(::[α, ::[::[id m.succ, Ty m], ::[id m.succ, Ty m]]]).snd
+
+.snd kind of normalizes, since it turns ((x : α) × (β x)) into just β x. it's normalization.
+
+snd is application.
+
+so, snd gives us like the output type. this is fine for the α → α part.
+but then what about x?
+
+nil feels like we can change it a bit.
+it downgrades us from a term to a type.
+
+nil.{[m]} α : α → (Ty m)
+nil α x = α
+
+::[x, α, ::[
+
+.snd.fst gives us the "assertion" for the given argument.
+.snd.snd gives us the return type.
+
+nil.{[m.succ]} (Ty m)
+
+::[(α : Ty m), ::[nil.{[m.succ]} (Ty m), ::[nil.{[m]}, ::[id m.succ, Ty m]]]
+
+::[nil.{[m.succ]} (Ty m), ::[nil.{[m]}, ::[id m.succ, Ty m]]
+nil.{[m]} α x = α
+::[α, ::[id m.succ, Ty m]]
+
+
+-/
